examples/backend/main.ml
@@ -1,13 +1,13 @@
 let compile name x = 
   let t = Unix.gettimeofday () in 
-  Printf.printf "Compilation of %s\n%!";
+  Printf.printf "Compilation of %s\n%!" name;
   match x with 
     Some x ->       
       Backend.dump (Backend.mk_block name x);
       Printf.printf "done (%fs)\n%!" (Unix.gettimeofday () -. t)
   | None -> Format.printf "Failed"
 
-let _ = compile "Cpu" Driver.example1
-let _ = compile "Adder" Driver.example2 
+(* A low key way to batch compile each one of our examples *)
+let _ = compile "Adder" Driver.example1 
+let _ = compile "Sorter" Driver.example2
 let _ = compile "Stack" Driver.example3
-let _ = compile "Sorter" Driver.example4
