src/Compiler.v
@@ -1,53 +1,35 @@
-Require Core Front IR RTL CSE CP FirstOrder (* DCE *). 
+Add Rec LoadPath "./" as Synthesis.
 
 
-Definition front Phi t  (a : forall Var, Front.action Phi Var t) : RTL.Block Phi t :=
+Require Core Front IR RTL CSE CP FirstOrder.
+
+
+Definition fesic Phi t  (a : forall Var, Front.action Phi Var t) : RTL.Block Phi t :=
   let x := IR.Compile Phi  t a in
   let x := RTL.Compile Phi t x in 
-  let x := CSE.Compile Phi t  x in  
-        x. 
+  let x := CSE.Compile Phi t  x in    
+  CP.Compile Phi t x.                 (* We use the notation BDD.compile in the paper here *)
 
-Definition opt Phi t (x : RTL.Block Phi t) (* :  option (FirstOrder.block Phi t) *) :=
-  let x := CP.Compile Phi t x in
-    (* Constant propagation may have introduced some extra sharing,
-    and we may have to remove some occurences of Evar *)
-  let x := CSE.Compile Phi t x in
-  x. 
+
+
 
 Axiom HWF : forall Phi t p, RTL.WF Phi t p. 
-Lemma front_correct (Phi : Core.state) t a :
-  let block := front Phi t a in 
-  forall st Delta, 
-    RTL.Eval Phi st t block Delta =
-    Front.Eval Phi st t a Delta. 
+Lemma fesic_correct (Phi : Core.state) t a :
+  let block := fesic Phi t a in 
+  forall st, 
+    RTL.Next Phi st t block =
+    Front.Next Phi st a. 
 Proof.
-  unfold front. intros. 
-  rewrite CSE.Compile_correct. 
+  unfold fesic. intros. 
+  rewrite CP.Compile_correct by apply HWF.  
+  rewrite CSE.Compile_correct by apply HWF. 
   rewrite RTL.Compile_correct. 
   rewrite IR.Compile_correct. 
   reflexivity. 
-  apply HWF. 
 Qed. 
 
-Lemma opt_correct (Phi : Core.state) t src :
-  let tgt := opt _ _ src in 
-  forall st Delta, 
-    RTL.Eval Phi st t tgt Delta =
-    RTL.Eval Phi st t src Delta. 
-Proof. 
-  unfold opt; intros. 
-  rewrite CSE.Compile_correct by apply HWF.  
-  rewrite CP.Compile_correct by apply HWF.  
-  reflexivity. 
-Qed.   
-
-Definition fesic Phi t src := 
-  let x := (front Phi t src) in 
+Definition Fesic Phi t src := 
+  let x := (fesic Phi t src) in 
   let x := FirstOrder.compile Phi t (x _ ) in 
-  (* DCE.compile Phi   *) Some x.
+  Some x.
  
-Definition fesiopt Phi t x := 
-  let x := opt Phi t (front Phi t x) in 
-  let x := FirstOrder.compile Phi t (x _ ) in 
-  (* DCE.compile Phi   *) Some x.
-
