examples/Driver.v
@@ -1,6 +1,5 @@
-Require Isa Add Stack Sorter.
+Require Add Stack Sorter.
 
-Definition example1 := Isa.t. 
-Definition example2 := (Compiler.fesiopt _ _  (Add.test 2)).
+Definition example1 := (Compiler.Fesic _ _  (Add.test 2)).
+Definition example2 := Sorter.t.
 Definition example3 := Stack.t.
-Definition example4 := Sorter.t.
