src/README.txt
@@ -1,0 +1,11 @@
+These files contain the compiler part of the development associated
+with the paper "Formal verification of Hardware Synthesis". 
+
+Running make in this directory will compile this development. However,
+in order to visit these files, one must either
+- run coqtop, and execute the command 
+  Add Rec LoadPath "./" as Synthesis.
+- run coqtop with the option 
+  -R "path_to_the_src_folder" "Synthesis"
+
+
